add semantics and fsim records for most Untyped passes

src/Untyped6.v
@@ -210,3 +210,26 @@ all: try solve [right; inversion 1; on >expr_value, invc].
 
 - finish_mut_induction value_dec using list.
 Qed.
+
+
+
+(* semantics *)
+
+Definition env := list expr.
+Definition prog_type : Type := list expr * list metadata.
+Definition valtype := value.
+
+Definition initial_env (prog : prog_type) : env := fst prog.
+
+Inductive is_callstate (prog : prog_type) : valtype -> valtype -> state -> Prop := .
+(* TODO: stub *)
+
+Inductive final_state (prog : prog_type) : state -> valtype -> Prop :=
+| FinalState : forall v, final_state prog (Stop v) v.
+
+Definition semantics (prog : prog_type) : Semantics.semantics :=
+  @Semantics_gen state env valtype
+                 (is_callstate prog)
+                 (sstep)
+                 (final_state prog)
+                 (initial_env prog).
