src/UntypedComp8.v
@@ -264,3 +264,69 @@ all: try on (I_expr _ be), invc.
     i_lem Forall2_length.
   + i_ctor. i_lem I_unroll_elim. i_ctor.
 Qed.
+
+
+
+Lemma compile_I_expr : forall a b,
+    compile_expr a = b ->
+    I_expr a b.
+mut_induction a using A.expr_rect_mut' with
+    (Pl := fun a => forall b,
+        compile_expr_list a = b ->
+        Forall2 I_expr a b);
+[ intros0 Hcomp; subst b; simpl in *; fold compile_expr_list; try i_ctor.. | ].
+
+- finish_mut_induction compile_I_expr using list.
+Qed exporting.
+
+Lemma compile_genv_I_expr : forall A B,
+    compile_genv A = B ->
+    Forall2 I_expr A B.
+intros. i_lem compile_I_expr_list.
+Qed.
+
+Lemma compile_cu_I_expr : forall A Ameta B Bmeta,
+    compile_cu (A, Ameta) = (B, Bmeta) ->
+    Forall2 I_expr A B.
+simpl. inversion 1. i_lem compile_genv_I_expr.
+Qed.
+
+Lemma I_expr_value : forall v a b,
+    I_expr a b ->
+    A.expr_value a v ->
+    B.expr_value b v.
+induction v using value_rect_mut with
+    (Pl := fun vs => forall as_ bs,
+        Forall2 I_expr as_ bs ->
+        Forall2 A.expr_value as_ vs ->
+        Forall2 B.expr_value bs vs);
+intros0 II Aev; invc Aev; invc II; i_ctor.
+Qed.
+
+Section Preservation.
+
+    Variable aprog : A.prog_type.
+    Variable bprog : B.prog_type.
+
+    Hypothesis Hcomp : compile_cu aprog = bprog.
+
+    Theorem fsim : Semantics.forward_simulation (A.semantics aprog) (B.semantics bprog).
+    destruct aprog as [A Ameta], bprog as [B Bmeta].
+    fwd eapply compile_cu_I_expr; eauto.
+
+    eapply Semantics.forward_simulation_step with
+        (match_states := I)
+        (match_values := @eq value).
+
+    - simpl. admit. (* callstate matching *)
+
+    - simpl. intros0 II Afinal. invc Afinal. invc II.
+      eexists. split. i_ctor. i_lem I_expr_value. i_ctor.
+
+    - intros0 Astep. intros0 II.
+      i_lem I_sim.
+
+    Admitted.
+
+End Preservation.
+
